Veir/IR/Dominance.lean
@@ -207,4 +207,22 @@ partial def opsInDominanceOrder
 
 end OperationPtr
 
+namespace ValuePtr
+
+/--
+Does the definition of `value` properly dominate the use of it by `op`?
+-/
+def properlyDominatesUse
+    (value : ValuePtr)
+    (op : OperationPtr)
+    (dfCtx : DataFlowContext)
+    (irCtx : WfIRContext OpCode) : Bool :=
+  match value with
+  | .opResult result =>
+      result.op.properlyDominates op dfCtx irCtx
+  | .blockArgument argument =>
+      (InsertPoint.atStart! argument.block irCtx.raw).dominates (.before op) dfCtx irCtx
+
+end ValuePtr
+
 end Veir
